theories/Compositional_Structures/Sepref_Bindings.thy
@@ -4,6 +4,7 @@ theory Sepref_Bindings
     "Basic_Modules/Component_Types/Defer_Equal_Condition_Ref"
     Sequential_Composition_Ref
     "../Borda_Rule_Ref"
+    "../Pairwise_Majority_Rule_Ref"
 
 begin
 
@@ -26,28 +27,11 @@ lemma condorcet_aux:
   done
 
 
-sepref_decl_op  (no_def) "borda :: 'a::{default, heap, hashable} Electoral_Module" 
-  ::  "elec_mod_rel_orig R" where "R = Id"
-    apply standard
-  apply (rule nres_relI)
-  apply simp done
-
-sepref_decl_op  (no_def) "elect_module :: 'a::{default, heap, hashable} Electoral_Module" 
-  ::  "elec_mod_rel_orig R" where "R = Id"
-  .
-
-(*sepref_decl_op  (no_def) condorcet ::  "elec_mod_rel_orig R" where "R = Id"
-    apply standard
-  apply (rule nres_relI)
-  apply simp done*)
-
-
-
-
 sepref_decl_op (no_def) defer_equal_imp: "(defer_equal_condition)" :: 
   "\<langle>nat_rel, \<langle>(\<langle>R\<rangle>set_rel \<times>\<^sub>r \<langle>R\<rangle>set_rel \<times>\<^sub>r \<langle>R\<rangle>set_rel), \<langle>bool_rel\<rangle>nres_rel\<rangle>fun_rel\<rangle>fun_rel" 
   where "R = Id" .
-                       
+
+
 
 locale refine_assns =
  notes  
@@ -55,62 +39,20 @@ locale refine_assns =
        alts_ref_assn_def[symmetric,fcomp_norm_unfold] 
        ballot_ref_assn_def[symmetric,fcomp_norm_unfold]
        alts_assn_def[symmetric,fcomp_norm_unfold] 
-      
 begin
 
 
 
-
-
-end
-
-locale sequence_sepref_direct = refine_assns +
- fixes m :: "'a::{default, heap, hashable} Electoral_Module"  and
-  n :: "'a::{default, heap, hashable} Electoral_Module"
-  fixes m_sep :: "'a::{default, heap, hashable} Electoral_Module_Sep" 
-  and n_sep :: "'a::{default, heap, hashable} Electoral_Module_Sep" 
-  assumes module_m: "electoral_module m"
-  and module_n: "electoral_module n"
-  and m_sep_correct: "(uncurry m_sep, uncurry ( RETURN oo m)) \<in> elec_mod_sep_rel id_assn"
-  and n_sep_correct: "(uncurry n_sep, uncurry ( RETURN oo n)) \<in> elec_mod_sep_rel id_assn"
-begin
-
-                                                              
-fun sequential_composition'' :: "'a::{default, heap, hashable} Electoral_Module \<Rightarrow> 
-      'a::{default, heap, hashable} Electoral_Module \<Rightarrow>
-        'a::{default, heap, hashable} set \<Rightarrow> 'a::{default, heap, hashable} Profile 
-\<Rightarrow> 'a::{default, heap, hashable} Result nres" where
-  "sequential_composition'' ma na A pr = do {
-      (mel,mrej,mdef) <- mop_borda A pr;
-      
-      let newA = mdef;
-      new_p <- mop_limit_profile newA pr;
-    
-      (nel,nrej,ndef) <- mop_elect_module newA new_p;
-      
-      RETURN (mel \<union> nel, mrej \<union> nrej, ndef)
-}"
-
-sepref_decl_impl borda_elim_sep.refine[FCOMP borda_ref_correct, sepref_fr_rules] 
-  by simp        
-
-sepref_decl_impl elect_elect_module_sep_correct [sepref_fr_rules]
-  by simp           
-
-
-sepref_definition seqcompd is "uncurry (RETURN oo (sequential_composition'
-  elect_module borda))"
-  :: "[\<lambda>(a, b).
-           finite a ]\<^sub>a (alts_set_impl_assn id_assn)\<^sup>k *\<^sub>a 
-    (list_assn (hr_comp (ballot_impl_assn id_assn) ballot_rel))\<^sup>k 
-        \<rightarrow> (result_impl_assn id_assn)"
-  unfolding sequential_composition'.simps 
+sepref_definition borda_rule_sep is "uncurry (seq_opt borda elect_module
+  )"
+  :: "[\<lambda>(x, xa).
+       finite
+        x]\<^sub>a (hs.assn nat_assn)\<^sup>k *\<^sub>a
+             (list_assn (hr_comp (ballot_impl_assn nat_assn) ballot_rel))\<^sup>k \<rightarrow> 
+  result_impl_assn  nat_assn"
+  unfolding seq_opt_def
   apply sepref_dbg_keep
- apply sepref_dbg_trans_keep
-  oops
-  
-
-end
+  done
 
 
 definition "impls \<equiv> borda_ref {1::nat, 2} ((([] @ [1::nat])@ [2::nat]) # [])"
@@ -123,22 +65,44 @@ definition "impls \<equiv> borda_ref {1::nat, 2} ((([] @ [1::nat])@ [2::nat]) # 
    apply (rewrite in "[(rewrite_HOLE @ [1::nat])@ [2::nat]]" arl.fold_custom_empty)
    apply (rewrite in "_ # rewrite_HOLE" HOL_list.fold_custom_empty)
    apply sepref_dbg_keep
-   done
+   done oops
 
 
 
-definition "dimpls \<equiv> borda {1::nat, 2} [{(1::nat, 2)}]"
+definition "dimpls A p \<equiv> do {
+  let (e, r, d) = borda A p;
+  ASSERT (finite d);
+  let newA = d;
+  let newp = limit_profile newA p;
+  let (ne, nr, nd) = elect_module newA newp;
+   RETURN (e \<union> ne, r \<union> nr, nd) }"
 
  sepref_definition second_imple 
-    is "uncurry0 (RETURN dimpls)" ::
- "unit_assn\<^sup>k \<rightarrow>\<^sub>a ( hr_comp (hs.assn id_assn) (\<langle>Id\<rangle>set_rel) \<times>\<^sub>a
-                   hr_comp (hs.assn id_assn) (\<langle>Id\<rangle>set_rel) \<times>\<^sub>a
-                   hr_comp (hs.assn id_assn) (\<langle>Id\<rangle>set_rel) )"
-   unfolding  dimpls_def comp_def
+    is "uncurry (dimpls)" ::
+    " [\<lambda>(a, b).
+           finite
+            a]\<^sub>a (alts_set_impl_assn nat_assn)\<^sup>k *\<^sub>a
+                 (list_assn
+                   (hr_comp (ballot_impl_assn nat_assn)
+                     ballot_rel))\<^sup>k \<rightarrow> result_impl_assn  nat_assn"
+   unfolding  dimpls_def aux_set_copy_def hs.fold_custom_empty
    apply sepref_dbg_keep
-apply sepref_dbg_trans_keep
    done
 
+lemma seqcomp_opt_correct: 
+  fixes m n :: "'a::{default,hashable,heap} Electoral_Module" and
+        A :: "'a set" and p :: "'a Profile"
+  assumes finprofa: "finite_profile A p" and
+   em_m: "electoral_module m" and
+  em_n: "electoral_module n"
+  shows "seq_opt m n A p \<le>
+   RETURN (sequential_composition' m n A p)"
+  unfolding comp_apply seq_opt_def sequential_composition'.simps
+ using assms apply (refine_vcg)
+   apply auto
+  by (metis def_presv_fin_prof snd_conv)
+
+end
 
 
 end
